Heaps are ordered now

experiments/SimplePar.v
@@ -24,17 +24,6 @@ Polymorphic Definition joinM@{d c}
 
 Hint Unfold joinM.
 
-Module Import M := FMapList.Make(Nat_as_OT).
-
-Definition add_with {A} (f : A -> A -> A) (key : nat) (new_val : A) (m : M.t A) : M.t A :=
-  match find key m with
-  | None => add key new_val m
-  | Some old_val => add key (f new_val old_val) m
-  end.
-
-Definition singleton {A} (key : nat) (val : A) : M.t A :=
-  M.add key val (M.empty A).
-
 Fixpoint split_at {A} (n : nat) (xs : list A) : list A * list A :=
   match (n, xs) with
   | (O, xs) => (nil, xs)
@@ -54,7 +43,90 @@ Module SimplePar.
 
 Definition Val := nat.
 
+Module Val_as_OT := Nat_as_OT.
+
 Definition IVar (A : Type) := nat.
+
+Module IVar_as_OT <: OrderedType.
+  Parameter A : Type.
+  Definition t := IVar A.
+  Definition eq := Nat_as_OT.eq.
+  Definition eq_refl := Nat_as_OT.eq_refl.
+  Definition eq_sym := Nat_as_OT.eq_sym.
+  Definition eq_trans := Nat_as_OT.eq_trans.
+  Definition lt := Nat_as_OT.lt.
+  Definition lt_trans := Nat_as_OT.lt_trans.
+  Definition lt_not_eq := Nat_as_OT.lt_not_eq.
+  Definition compare := Nat_as_OT.compare.
+  Definition eq_dec := Nat_as_OT.eq_dec.
+End IVar_as_OT.
+
+Module option_as_OT (A : OrderedType) <: OrderedType.
+  Module OA := OrderedTypeFacts (A).
+  Definition t:= option A.t.
+  Definition eq x y :=
+    match (x, y) with
+    | (None, None) => True
+    | (None, Some y) => False
+    | (Some x, None) => False
+    | (Some x, Some y) => A.eq x y
+    end.
+  Hint Unfold eq.
+  Ltac crush_eq :=
+    repeat match goal with
+           | [ H : t |- _] => destruct H
+           | [ H : eq None (Some _) |- _] => inversion H
+           | [ H : eq (Some _) None |- _] => inversion H
+           | _ => eauto
+           end.
+  Definition eq_refl : forall x : t, eq x x.
+    intros; crush_eq.
+  Qed.
+  Definition eq_sym : forall x y : t, eq x y -> eq y x.
+    intros; crush_eq.
+  Qed.
+  Definition eq_trans : forall x y z : t, eq x y -> eq y z -> eq x z.
+    intros; crush_eq.
+  Qed.
+  Definition lt (x y : t) :=
+    match (x, y) with
+    | (None, None) => False
+    | (None, Some y) => True
+    | (Some x, None) => False
+    | (Some x, Some y) => A.lt x y
+    end.
+  Hint Unfold lt.
+  Ltac crush_lt :=
+    repeat match goal with
+           | [ H : t |- _] => destruct H
+           | [ H : lt (Some _) None |- _] => inversion H
+           | [ H : eq (Some _) None |- _] => inversion H
+           | [ H : eq None (Some _) |- _] => inversion H
+           | [ H : lt _ _ |- ~ _] => eapply A.lt_not_eq in H
+           | [ |- Compare _ _ None None] => eapply EQ
+           | [ |- Compare _ _ None (Some _)] => eapply LT
+           | [ |- Compare _ _ (Some _) None] => eapply GT
+           | [ H : A.lt ?X ?Y |- Compare _ _ (Some ?X) (Some ?Y)] => eapply LT
+           | [ H : A.eq ?X ?Y |- Compare _ _ (Some ?X) (Some ?Y)] => eapply EQ
+           | [ H : A.lt ?Y ?X |- Compare _ _ (Some ?X) (Some ?Y)] => eapply GT
+           | [ |- {eq ?X ?Y} + {~ eq ?X ?Y}] => unfold eq
+           | [ |- {A.eq ?X ?Y} + {~ A.eq ?X ?Y}] => eapply A.eq_dec
+           | _ => eauto
+           end.
+  Definition lt_trans : forall x y z : t, lt x y -> lt y z -> lt x z.
+    intros; crush_lt.
+  Qed.
+  Definition lt_not_eq : forall x y : t, lt x y -> ~ eq x y.
+    intros; crush_lt.
+  Qed.
+  Definition compare : forall x y : t, Compare lt eq x y.
+    intros [x|] [y|]. destruct (A.compare x y).
+    all: crush_lt.
+  Qed.
+  Definition eq_dec : forall x y : t, {eq x y} + {~ eq x y}.
+    intros; crush_lt.
+  Qed.
+End option_as_OT.
 
 Inductive Trace : Type :=
   Get  : IVar Val -> (Val -> Trace) -> Trace
@@ -102,6 +174,26 @@ Definition fork (p : Par unit) : Par unit :=
   | mkPar k1 => mkPar (fun k2 => Fork (k1 (fun _ => Done)) (k2 tt))
   end.
 
+Module OV_as_OT := option_as_OT Val_as_OT.
+
+Module H := FMapList.Make_ord Nat_as_OT OV_as_OT.
+Module HM := H.MapS.
+
+Definition Heap := H.t.
+
+Module M := FMapList.Make (Nat_as_OT).
+
+Definition add_with {A} (f : A -> A -> A) (key : nat) (new_val : A) (m : M.t A) : M.t A :=
+  match M.find key m with
+  | None => M.add key new_val m
+  | Some old_val => M.add key (f new_val old_val) m
+  end.
+
+Definition singleton {A} (key : nat) (val : A) : HM.t A :=
+  HM.add key val (HM.empty A).
+
+Definition Pool := M.t (list (Val -> Trace)).
+
 Inductive Exn : Type :=
   MultiplePut : Val -> nat -> Val -> Exn
 | Deadlock : M.t (list (Val -> Trace)) -> Exn
@@ -109,23 +201,19 @@ Inductive Exn : Type :=
 | OutOfFuel : Exn
 .
 
-Definition Heap := M.t (option Val).
-
-Definition Pool := M.t (list (Val -> Trace)).
-
 Definition step (trc : Trace) (others : list Trace)
            (blkd : Pool) (cntr : nat) (heap : Heap)
   : Exn + (list Trace * Pool * nat * Heap) :=
   match trc with
   | Done => ret (others, blkd, cntr, heap)
   | Fork t1 t2 => ret (t1 :: t2 :: others, blkd, cntr, heap)
-  | New k => ret (k cntr :: others, blkd, cntr + 1, M.add cntr None heap)
-  | Get ix k => match joinM (M.find ix heap) with
+  | New k => ret (k cntr :: others, blkd, cntr + 1, HM.add cntr None heap)
+  | Get ix k => match joinM (HM.find ix heap) with
                | None => ret (others, add_with (app (A:=_)) ix [k] blkd, cntr, heap)
                | Some v => ret (k v :: others, blkd, cntr, heap)
                end
-  | Put ix v t2 => let heap' := M.add ix (Some v) heap in
-                  match joinM (M.find ix heap) with
+  | Put ix v t2 => let heap' := HM.add ix (Some v) heap in
+                  match joinM (HM.find ix heap) with
                   | None => match M.find ix blkd with
                            | None => ret (t2 :: others, blkd, cntr, heap')
                            | Some ls => ret (t2 :: fmap (fun k => k v) ls ++ others, M.remove ix blkd, cntr, heap')
@@ -157,7 +245,7 @@ Definition runPar (randoms : Stream nat) (p : Par Val) : Exn + Val :=
   let initThreads := [ runCont p (fun v => Put 0 v Done) ] in
   let maxFuel := 100 in
   finalHeap <- sched maxFuel randoms initThreads (M.empty _) 1 initHeap ;;
-  match joinM (M.find 0 finalHeap) with
+  match joinM (HM.find 0 finalHeap) with
   | None => inl HeapExn
   | Some finalVal => ret finalVal
   end
@@ -194,6 +282,11 @@ Example dag1 : Par Val :=
 
 Eval cbn in runPar canonical dag1.
 Eval cbn in runPar round_robin dag1.
+
+Example heap1 : Heap := singleton 0 None.
+Example heap2 : Heap := singleton 0 (Some 1).
+
+Eval cbv in H.lt heap1 heap2.
 
 (* Fixpoint loopit {A} (acc : Val) (vr : IVar Val) : Par A := *)
 (*   bind (get vr) (fun n => loopit (acc + n) vr). *)
